more

Weidenbach_Book/Watched_Literals_Algorithm_Enumeration.thy
@@ -8,54 +8,103 @@ definition cdcl_twl_enum_inv where
 definition equisatisfiable :: \<open>'v clauses \<Rightarrow> 'v clauses \<Rightarrow> bool\<close> where
 \<open>equisatisfiable N N' \<longleftrightarrow> (\<forall>M. M \<Turnstile>sm N \<longleftrightarrow> M \<Turnstile>sm N')\<close>
 
-definition enum_equisatisfiable_st_clss :: \<open>('v twl_st \<times> 'v clauses) set\<close> where
-  \<open>enum_equisatisfiable_st_clss = {(S, N). equisatisfiable (clauses (get_clauses S)) N}\<close>
+definition enum_equisatisfiable_st_clss :: \<open>('v twl_st \<times> ('v literal list option \<times> 'v clauses)) set\<close> where
+  \<open>enum_equisatisfiable_st_clss = {(S, (M, N)). equisatisfiable (clauses (get_clauses S)) N}\<close>
 
-definition enum_model_st :: \<open>('v twl_st \<times> 'v literal list option) set\<close> where
-  \<open>enum_model_st = {(S, M).
+definition enum_model_st :: \<open>('v twl_st \<times> ('v literal list option \<times> 'v clauses)) set\<close> where
+  \<open>enum_model_st = {(S, (M, N)).
+         equisatisfiable (add_mset (DECO_clause (get_trail S)) (clauses (get_clauses S))) N \<and>
          (get_conflict S \<noteq> None \<longrightarrow> M \<noteq> None \<and> lits_of_l (get_trail S) = set (the M)) \<and>
          (get_conflict S = None \<longrightarrow> M = None)}\<close>
 
+
+fun add_to_init_cls :: \<open>'v twl_cls \<Rightarrow> 'v twl_st \<Rightarrow> 'v twl_st\<close> where
+  \<open>add_to_init_cls C (M, N, U, D, NE, UE, WS, Q) = (M, add_mset C N, U, D, NE, UE, WS, Q)\<close>
 
 context
   fixes P :: \<open>'v literal set \<Rightarrow> bool\<close>
 begin
 
-definition cdcl_twl_enum :: \<open>'v twl_st \<Rightarrow> 'v twl_st nres\<close>where
+definition cdcl_twl_enum :: \<open>'v twl_st \<Rightarrow> 'v twl_st nres\<close> where
   \<open>cdcl_twl_enum S = do {
      S \<leftarrow> conclusive_TWL_run S;
      WHILE\<^sub>T\<^bsup>cdcl_twl_enum_inv\<^esup>
        (\<lambda>S. get_conflict S \<noteq> None \<and> P (lits_of_l (get_trail S)))
-       (\<lambda>S. conclusive_TWL_run S)
+       (\<lambda>S. do {
+             S \<leftarrow> SPEC (negate_model_and_add S);
+             conclusive_TWL_run S
+           })
        S
     }\<close>
 
-lemma enumerate_model_unless_alt_def:
-  \<open>RETURN (enumerate_model_unless P N) = do {
-     let MN = (N, get_option_model N);
-     (N, M) \<leftarrow> WHILE\<^sub>T (\<lambda>(N, M). M \<noteq> None \<and> \<not>P (set (the M)))
-       (\<lambda>(N, M). do {
-          let C = (image_mset uminus (mset (the M)));
-          RETURN (add_mset C N, get_option_model (add_mset C N))
-        })
-       MN;
-     RETURN M
-   }\<close>
-  apply (induction P N rule: enumerate_model_unless.induct)
-  apply (subst enumerate_model_unless.simps)
-  apply (subst WHILET_unfold)
-  apply (auto split: option.splits)
-  done
+definition next_model_filtered_nres where
+  \<open>next_model_filtered_nres N = 
+    SPEC (\<lambda>M. full (next_model_filtered P) N M)\<close>
 
 lemma
-  \<open>(cdcl_twl_enum, RETURN o (enumerate_model_unless P)) \<in> 
+  \<open>(cdcl_twl_enum, next_model_filtered_nres) \<in> 
     enum_equisatisfiable_st_clss \<rightarrow>\<^sub>f \<langle>enum_model_st\<rangle>nres_rel\<close>
-  unfolding cdcl_twl_enum_def enum_equisatisfiable_st_clss_def
-  apply (intro frefI nres_relI)
-  apply simp
-  apply (subst enumerate_model_unless_alt_def[abs_def])
-  apply clarify
-  apply refine_vcg
+proof -
+  define model_if_exists where
+    \<open>model_if_exists S \<equiv> \<lambda>M. 
+      (if no_step (next_model_filtered P) S then M=S else next_model_filtered P S M)\<close>
+      for S :: \<open>_ \<times> 'v clauses\<close>
+  have \<open>full (next_model_filtered P) S U \<longleftrightarrow>  
+         (\<exists>T. model_if_exists S T \<and> full (next_model_filtered P) T U)\<close> (is \<open>?A \<longleftrightarrow> ?B\<close>)
+    for S U
+  proof
+    assume ?A
+    then consider
+      (nss) \<open>no_step (next_model_filtered P) S\<close> |
+      (s1) T where \<open>(next_model_filtered P) S T\<close> and \<open>full (next_model_filtered P) T U\<close>
+      unfolding full_def
+      by (metis converse_rtranclpE)
+    then show ?B
+    proof cases
+      case nss
+      then have \<open>model_if_exists S S\<close>
+        unfolding model_if_exists_def by simp
+      then show ?B
+        using \<open>?A\<close> by blast
+    next
+      case (s1 T)
+      then have \<open>model_if_exists S T\<close>
+        unfolding model_if_exists_def
+        by meson
+      then show ?B
+        using s1 by blast
+    qed
+  next
+    assume ?B
+    then show ?A
+      by (auto simp: model_if_exists_def full1_is_full full_fullI split: if_splits)
+  qed
+  then have next_model_filtered_nres_alt_def: \<open>next_model_filtered_nres  = (\<lambda>S. do {
+         S \<leftarrow> SPEC (model_if_exists S);
+         SPEC (\<lambda>T. full (next_model_filtered P) S T)
+       })\<close>
+    apply (intro ext)
+    unfolding next_model_filtered_nres_def (* model_if_exists_def *) RES_RES_RETURN_RES
+    by fast
+  have \<open>conclusive_TWL_run S
+      \<le> \<Down> enum_model_st
+          (SPEC (model_if_exists MN))\<close>
+    if
+      \<open>(S, MN) \<in> {(S, M, y). equisatisfiable (clauses (get_clauses S)) y}\<close>
+    for S MN
+  proof -
+    show ?thesis
+      unfolding conclusive_TWL_run_def
+      apply (auto simp: enum_model_st_def RES_refine
+          intro!: RES_refine)
+      sorry
+  qed
+  show ?thesis
+    unfolding cdcl_twl_enum_def enum_equisatisfiable_st_clss_def  next_model_filtered_nres_alt_def
+    apply (intro frefI nres_relI)
+    apply refine_vcg
+    subgoal for S MN
+      explore_have
   oops
 
 end
